coq/JsPrettyRules.v
@@ -735,7 +735,7 @@ with red_expr : state -> execution_ctx -> ext_expr -> out -> Prop :=
   | red_expr_object_1_nil : forall S C l,
       red_expr S C (expr_object_1 l nil) (out_ter S l)
   
-  | red_expr_object_1_cons : forall S0 S C x l pn pb pds o, 
+  | red_expr_object_1_cons : forall S C x l pn pb pds o, 
       x = string_of_propname pn ->
       red_expr S C (expr_object_2 l x pb pds) o ->
       red_expr S C (expr_object_1 l ((pn,pb)::pds)) o
@@ -760,7 +760,7 @@ with red_expr : state -> execution_ctx -> ext_expr -> out -> Prop :=
       red_expr S C (expr_object_4 l x A pds) o ->
       red_expr S0 C (expr_object_3_get l x (out_ter S v) pds) o
 
-  | red_expr_object_2_set : forall S S0 C l x v pds o o1 bd args,
+  | red_expr_object_2_set : forall S C l x pds o o1 bd args,
       red_expr S C (spec_create_new_function_in C args bd) o1 ->
       red_expr S C (expr_object_3_set l x o1 pds) o ->
       red_expr S C (expr_object_2 l x (propbody_set args bd) pds) o
@@ -770,12 +770,12 @@ with red_expr : state -> execution_ctx -> ext_expr -> out -> Prop :=
       red_expr S C (expr_object_4 l x A pds) o ->
       red_expr S0 C (expr_object_3_set l x (out_ter S v) pds) o
   
-  | red_expr_object_4_define_own_prop : forall S S0 C A l x v pds o o1,
+  | red_expr_object_4 : forall S S0 C A l x pds o o1,
       red_expr S C (spec_object_define_own_prop l x A false) o1 ->
       red_expr S C (expr_object_5 l pds o1) o ->
       red_expr S C (expr_object_4 l x A pds) o
 
-  | red_expr_object_5_next_property : forall S S0 rv C A l x v pds o,
+  | red_expr_object_5 : forall S S0 C rv l pds o,
       red_expr S C (expr_object_1 l pds) o ->
       red_expr S0 C (expr_object_5 l pds (out_ter S rv)) o   
 
